Split up Iris modules further; updated all instantiations; [MinCaps] Expr relation succesfully implemented

case_study/MinimalCaps/Model.v
@@ -90,82 +90,102 @@ Module MinCapsModel.
   Import MinCapsProgram.
   Import MinCapsSpecification.
 
-  Module MinCapsIrisParams <: IrisParameters MinCapsBase MinCapsProgram MinCapsSignature MinCapsSemantics.
+  Module MinCapsIrisPrelims <: IrisPrelims MinCapsBase MinCapsProgram MinCapsSignature MinCapsSemantics.
+    Include IrisPrelims MinCapsBase MinCapsProgram MinCapsSignature MinCapsSemantics.
+  End MinCapsIrisPrelims.
 
-  Include IrisPrelims MinCapsBase MinCapsProgram MinCapsSignature MinCapsSemantics.
+  Module MinCapsIrisParams <: IrisParameters MinCapsBase MinCapsProgram MinCapsSignature MinCapsSemantics MinCapsIrisPrelims.
+    Import MinCapsIrisPrelims.
 
     Variable maxAddr : nat.
 
     Section WithIrisNotations.
+      Import iris.bi.interface.
+      Import iris.bi.big_op.
+      Import iris.base_logic.lib.iprop.
+      Import iris.base_logic.lib.gen_heap.
 
+      Definition MemVal : Set := Z + Capability.
+
+      Class mcMemGS Σ := McMemGS {
+                            (* ghost variable for tracking state of registers *)
+                            mc_ghG :> gh.gen_heapGS Z MemVal Σ;
+                            mc_invNs : namespace
+                          }.
+
+      Definition memGpreS : gFunctors -> Set := fun Σ => gh.gen_heapGpreS Z MemVal Σ.
+      Definition memGS : gFunctors -> Set := mcMemGS.
+      Definition memΣ : gFunctors := gh.gen_heapΣ Z MemVal.
+
+      Definition memΣ_GpreS : forall {Σ}, subG memΣ Σ -> memGpreS Σ :=
+        fun {Σ} => gh.subG_gen_heapGpreS (Σ := Σ) (L := Z) (V := MemVal).
+
+      Definition mem_inv : forall {Σ}, memGS Σ -> Memory -> iProp Σ :=
+        fun {Σ} hG μ =>
+          (∃ memmap, gen_heap_interp (hG := mc_ghG (mcMemGS := hG)) memmap ∗
+                                     ⌜ map_Forall (fun a v => μ a = v) memmap ⌝
+          )%I.
+
+      Definition liveAddrs : list Addr := seqZ 0 maxAddr.
+      Definition initMemMap μ := (list_to_map (map (fun a => (a , μ a)) liveAddrs) : gmap Addr MemVal).
+
+      Lemma initMemMap_works μ : map_Forall (λ (a : Addr) (v : MemVal), μ a = v) (initMemMap μ).
+      Proof.
+        unfold initMemMap.
+        rewrite map_Forall_to_list.
+        rewrite Forall_forall.
+        intros (a , v).
+        rewrite elem_of_map_to_list.
+        intros el.
+        apply elem_of_list_to_map_2 in el.
+        apply elem_of_list_In in el.
+        apply in_map_iff in el.
+        by destruct el as (a' & <- & _).
+      Qed.
+
+      Definition mem_res : forall {Σ}, memGS Σ -> Memory -> iProp Σ :=
+        fun {Σ} hG μ =>
+          ([∗ map] l↦v ∈ initMemMap μ, mapsto (hG := mc_ghG (mcMemGS := hG)) l (DfracOwn 1) v) %I.
+
+      Lemma mem_inv_init : forall Σ (μ : Memory), memGpreS Σ ->
+                                                  ⊢ |==> ∃ mG : memGS Σ, (mem_inv mG μ ∗ mem_res mG μ)%I.
+      Proof.
+        iIntros (Σ μ gHP).
+
+        iMod (gen_heap_init (gen_heapGpreS0 := gHP) (L := Addr) (V := MemVal) empty) as (gH) "[inv _]".
+        pose (memmap := initMemMap μ).
+        iMod (gen_heap_alloc_big empty memmap (map_disjoint_empty_r memmap) with "inv") as "(inv & res & _)".
+        iModIntro.
+
+        rewrite (right_id empty union memmap).
+
+        iExists (McMemGS gH (nroot .@ "addr_inv")).
+        iFrame.
+        iExists memmap.
+        iFrame.
+        iPureIntro.
+        apply initMemMap_works.
+      Qed.
+    End WithIrisNotations.
+  End MinCapsIrisParams.
+
+  Module MinCapsIrisResources <: IrisResources MinCapsBase MinCapsSignature MinCapsSemantics MinCapsIrisPrelims MinCapsIrisParams.
+    Include IrisResources MinCapsBase MinCapsSignature MinCapsSemantics MinCapsIrisPrelims MinCapsIrisParams.
+  End MinCapsIrisResources.
+
+
+  Section Predicates.
+    Import env.notations.
+    Import MinCapsIrisPrelims.
+    Import MinCapsIrisParams.
+    Import MinCapsIrisResources.
     Import iris.bi.interface.
     Import iris.bi.big_op.
     Import iris.base_logic.lib.iprop.
     Import iris.base_logic.lib.gen_heap.
+    Context {Σ} `{sailRegGS Σ} `{invGS Σ} {mG : memGS Σ}.
 
-    Definition MemVal : Set := Z + Capability.
-
-    Class mcMemGS Σ := McMemGS {
-                          (* ghost variable for tracking state of registers *)
-                          mc_ghG :> gh.gen_heapGS Z MemVal Σ;
-                          mc_invNs : namespace
-                        }.
-
-    Definition memGpreS : gFunctors -> Set := fun Σ => gh.gen_heapGpreS Z MemVal Σ.
-    Definition memGS : gFunctors -> Set := mcMemGS.
-    Definition memΣ : gFunctors := gh.gen_heapΣ Z MemVal.
-
-    Definition memΣ_GpreS : forall {Σ}, subG memΣ Σ -> memGpreS Σ :=
-      fun {Σ} => gh.subG_gen_heapGpreS (Σ := Σ) (L := Z) (V := MemVal).
-
-    Definition mem_inv : forall {Σ}, memGS Σ -> Memory -> iProp Σ :=
-      fun {Σ} hG μ =>
-        (∃ memmap, gen_heap_interp (hG := mc_ghG (mcMemGS := hG)) memmap ∗
-                                ⌜ map_Forall (fun a v => μ a = v) memmap ⌝
-        )%I.
-
-    Definition liveAddrs : list Addr := seqZ 0 maxAddr.
-    Definition initMemMap μ := (list_to_map (map (fun a => (a , μ a)) liveAddrs) : gmap Addr MemVal).
-
-    Lemma initMemMap_works μ : map_Forall (λ (a : Addr) (v : MemVal), μ a = v) (initMemMap μ).
-    Proof.
-      unfold initMemMap.
-      rewrite map_Forall_to_list.
-      rewrite Forall_forall.
-      intros (a , v).
-      rewrite elem_of_map_to_list.
-      intros el.
-      apply elem_of_list_to_map_2 in el.
-      apply elem_of_list_In in el.
-      apply in_map_iff in el.
-      by destruct el as (a' & <- & _).
-    Qed.
-
-    Definition mem_res : forall {Σ}, memGS Σ -> Memory -> iProp Σ :=
-      fun {Σ} hG μ =>
-        ([∗ map] l↦v ∈ initMemMap μ, mapsto (hG := mc_ghG (mcMemGS := hG)) l (DfracOwn 1) v) %I.
-
-    Lemma mem_inv_init : forall Σ (μ : Memory), memGpreS Σ ->
-      ⊢ |==> ∃ mG : memGS Σ, (mem_inv mG μ ∗ mem_res mG μ)%I.
-    Proof.
-      iIntros (Σ μ gHP).
-
-      iMod (gen_heap_init (gen_heapGpreS0 := gHP) (L := Addr) (V := MemVal) empty) as (gH) "[inv _]".
-      pose (memmap := initMemMap μ).
-      iMod (gen_heap_alloc_big empty memmap (map_disjoint_empty_r memmap) with "inv") as "(inv & res & _)".
-      iModIntro.
-
-      rewrite (right_id empty union memmap).
-
-      iExists (McMemGS gH (nroot .@ "addr_inv")).
-      iFrame.
-      iExists memmap.
-      iFrame.
-      iPureIntro.
-      apply initMemMap_works.
-    Qed.
-
-    Definition MinCaps_ptsreg `{sailRegGS Σ} (reg : RegName) (v : Z + Capability) : iProp Σ :=
+    Definition MinCaps_ptsreg (reg : RegName) (v : Z + Capability) : iProp Σ :=
       match reg with
       | R0 => reg_pointsTo reg0 v
       | R1 => reg_pointsTo reg1 v
@@ -173,7 +193,7 @@ Module MinCapsModel.
       | R3 => reg_pointsTo reg3 v
       end.
 
-    Lemma MinCaps_ptsreg_regtag_to_reg `{sailRegGS Σ} (reg : RegName) (v : Z + Capability) :
+    Lemma MinCaps_ptsreg_regtag_to_reg (reg : RegName) (v : Z + Capability) :
       MinCaps_ptsreg reg v = reg_pointsTo (regtag_to_reg reg) v.
     Proof.
       by destruct reg.
@@ -196,8 +216,11 @@ Module MinCapsModel.
       lia.
     Qed.
 
-    Context {Σ : gFunctors}.
+    (* Notation D := (MemVal -d> iPropO Σ).
+         Notation C := (Capability -d> iPropO Σ).
+         Implicit Type w : MemVal. *)
     Notation D := ((leibnizO MemVal) -n> iPropO Σ). (* TODO: try -d>, drop leibnizO, might not need λne *)
+    Notation C := ((leibnizO Capability) -n> iPropO Σ). (* TODO: try -d>, drop leibnizO, might not need λne *)
     Implicit Type w : (leibnizO MemVal).
 
     (* Copied from github.com/logsem/cerise *)
@@ -220,68 +243,113 @@ Module MinCapsModel.
 
     Definition GPRs : list RegName := finite.enum RegName.
 
-    Definition interp_gprs `{sailRegGS Σ} `{invGS Σ} `{mG : memGS Σ} (safe : D) : iProp Σ :=
-      [∗ list] r ∈ GPRs, (∃ w, MinCaps_ptsreg r w ∗ safe w)%I.
+    (* TODO:
+       - Make the change to D proposed above, might simplify some stuff
+         Need to look into what the difference induced by that change is...
+       - make the interp definitions more uniform, i.e., they should all take an
+         interp (= safe) and have return type D *)
+    Program Definition interp_gprs : D -n> iPropO Σ :=
+      λne interp, ([∗ list] r ∈ GPRs, (∃ w, MinCaps_ptsreg r w ∗ interp w))%I.
+    Solve Obligations with solve_proper.
 
-    Definition interp_expr `{sailRegGS Σ} `{invGS Σ} {mG : memGS Σ} (safe : D) (c : Capability) : iProp Σ :=
-      reg_pointsTo pc c ∗ interp_gprs (mG := mG) safe -∗ True. (* TODO: should be wp fdeCycle ⊤? *)
+    Definition interp_loop `{sg : sailGS Σ} : iProp Σ :=
+      (WP (MkConf (FunDef loop) env.nil) ?{{_, True}})%I.
 
-    Program Definition MinCaps_ref_inv `{sailRegGS Σ} `{invGS Σ} {mG : memGS Σ} (a : Addr) : D -n> iPropO Σ :=
+    Definition interp_expr (interp : D) : C :=
+      (λne (c : leibnizO Capability),
+        reg_pointsTo pc c ∗ interp_gprs interp -∗ (interp_loop (sg := SailGS _ _ mG)))%I.
+
+    (* TODO: Check if I tried changing this one to a discrete one, should remain non-expansive so we can proof contractiveness *)
+    Program Definition interp_ref_inv (a : Addr) : D -n> iPropO Σ :=
       λne P, (∃ w, mapsto (hG := mc_ghG (mcMemGS := mG)) a (DfracOwn 1) w ∗ P w)%I.
-    Solve All Obligations with solve_proper.
+    Solve Obligations with solve_proper.
 
-    Program Definition MinCaps_csafe `{sailRegGS Σ} `{invGS Σ} {mG : memGS Σ} (safe : D) : D :=
-      λne w,
-        (match w with
-        | inr (MkCap O b e a) => True%I
-        | inr (MkCap E b e a) => ▷ □ (interp_expr (mG := mG) safe (MkCap E b e a))
-        | inr (MkCap R b e a) =>
-          (⌜ (b <= e)%Z ⌝ →
-            ⌜ b ∈ liveAddrs /\ e ∈ liveAddrs ⌝ ∗
-                                [∗ list] a ∈ (region_addrs b e), inv (mc_invNs (mcMemGS := mG) .@ a) (MinCaps_ref_inv (mG := mG) a safe))
-          ∨
-          ⌜ (e < b)%Z ⌝
-        | inr (MkCap RW b e a) =>
-          (⌜ (b <= e)%Z ⌝ →
-            ⌜ b ∈ liveAddrs /\ e ∈ liveAddrs ⌝ ∗
-                                [∗ list] a ∈ (region_addrs b e), inv (mc_invNs (mcMemGS := mG) .@ a) (MinCaps_ref_inv (mG := mG) a safe))
-          ∨
-          ⌜ (e < b)%Z ⌝
-        | inl _ => False
-        end)%I.
+    Definition interp_cap_inv (c : Capability) (interp : D) :iProp Σ := 
+      match c with
+      | MkCap _ b e a =>
+          (⌜(b <= e)%Z⌝ →
+           ⌜b ∈ liveAddrs /\ e ∈ liveAddrs⌝ ∗
+                               [∗ list] a ∈ (region_addrs b e), inv (mc_invNs (mcMemGS := mG) .@ a) (interp_ref_inv a interp))
+          ∨ ⌜(e < b)%Z⌝
+      end.
 
-    Program Definition MinCaps_safe1 `{sailRegGS Σ} `{invGS Σ} {mG : memGS Σ} (safe : D) : D :=
-      λne w,
-        (match w with
-        | inl z => True
-        | inr c => MinCaps_csafe (mG := mG) safe w
-        end)%I.
+    Program Definition interp_cap_O : D := λne _, True%I.
 
-    Global Instance MinCaps_csafe_contractive `{sailRegGS Σ} `{invGS Σ} {mG : memGS Σ} :
-      Contractive (MinCaps_csafe (mG := mG)).
+    Program Definition interp_cap_R (interp : D) : D :=
+      λne w, (match w with
+              | inr (MkCap R b e a) => interp_cap_inv (MkCap R b e a) interp
+              | _                   => False
+              end)%I.
+    Solve Obligations with solve_proper.
+
+    Program Definition interp_cap_RW (interp : D) : D :=
+      λne w, (match w with
+              | inr (MkCap RW b e a) => interp_cap_inv (MkCap RW b e a) interp
+              | _                    => False
+              end)%I.
+    Solve Obligations with solve_proper.
+
+    Program Definition enter_cond (b e a : Addr) : D -n> iPropO Σ :=
+      λne interp, (▷ □ interp_expr interp (MkCap R b e a))%I.
+    Solve Obligations with solve_proper.
+
+    Program Definition interp_cap_E (interp : D) : D :=
+      λne w, (match w with
+              | inr (MkCap E b e a) => enter_cond b e a interp
+              | _                   => False
+              end)%I.
+    Solve Obligations with solve_proper.
+
+    Program Definition interp_z : D :=
+      λne w, ⌜ match w with
+               | inl _ => True
+               | _     => False
+               end ⌝%I.
+    Solve Obligations with solve_proper.
+
+    Definition interp1 (interp : D) : D :=
+      λne w, (match w with
+              | inl _                => interp_z w
+              | inr (MkCap O _ _ _)  => interp_cap_O w
+              | inr (MkCap R _ _ _)  => interp_cap_R interp w
+              | inr (MkCap RW _ _ _) => interp_cap_RW interp w
+              | inr (MkCap E _ _ _)  => interp_cap_E interp w
+              end)%I.
+
+    Global Instance interp_cap_O_contractive :
+      Contractive interp_cap_O.
+    Proof. solve_contractive. Qed.
+    Global Instance interp_cap_R_contractive :
+      Contractive interp_cap_R.
     Proof.
       intros n x y Hdist w.
-      unfold MinCaps_csafe.
-      destruct w; first by intuition.
-      destruct c.
-      destruct cap_permission; first auto; solve_proper_prepare; solve_contractive.
+      destruct w; auto.
+      destruct c; destruct cap_permission; solve_contractive.
     Qed.
-
-    Global Instance MinCaps_safe1_contractive `{sailRegGS Σ} `{invGS Σ} {mG : memGS Σ} :
-      Contractive (MinCaps_safe1 (mG := mG)).
+    Global Instance interp_cap_RW_contractive :
+      Contractive interp_cap_RW.
     Proof.
       intros n x y Hdist w.
-      unfold MinCaps_safe1.
-      destruct w; first by intuition.
-      by apply MinCaps_csafe_contractive.
+      destruct w; auto.
+      destruct c; destruct cap_permission; solve_contractive.
     Qed.
+    Global Instance interp_cap_E_contractive :
+      Contractive interp_cap_E.
+    Proof.
+      intros n x y Hdist w.
+      destruct w; auto.
+      destruct c; destruct cap_permission; solve_contractive.
+    Qed.
+    Global Instance interp1_contractive :
+      Contractive interp1.
+    Proof. solve_contractive. Qed.
 
-    Lemma fixpoint_MinCaps_safe1_eq `{sailRegGS Σ} `{invGS Σ} {mG : memGS Σ} (w : leibnizO MemVal) :
-      fixpoint (MinCaps_safe1 (mG := mG)) w ≡ MinCaps_safe1 (mG := mG) (fixpoint (MinCaps_safe1 (mG := mG))) w.
-    Proof. exact: (fixpoint_unfold (MinCaps_safe1 (mG := mG)) w). Qed.
+    Definition interp : D :=
+      λne w, (fixpoint (interp1)) w.
 
-    Definition MinCaps_safe `{sailRegGS Σ} `{invGS Σ} {mG : memGS Σ} : D :=
-      λne w, (fixpoint (MinCaps_safe1 (mG := mG))) w.
+    Lemma fixpoint_interp1_eq w :
+      fixpoint interp1 w ≡ interp1 (fixpoint interp1) w.
+    Proof. exact: (fixpoint_unfold interp1 w). Qed.
 
     Lemma le_liveAddrs (a b e : Addr) :
       b ∈ liveAddrs ∧ e ∈ liveAddrs ->
@@ -297,10 +365,10 @@ Module MinCapsModel.
       split; lia.
     Qed.
 
-    Lemma region_addrs_submseteq `{sailRegGS Σ} `{invGS Σ} {mG : memGS Σ} (b' e' b e : Addr) :
+    Lemma region_addrs_submseteq  (b' e' b e : Addr) :
       ⊢ ⌜ (b <= b')%Z /\ (e' <= e)%Z ⌝ -∗
-                               ([∗ list] a ∈ (region_addrs b e), inv (mc_invNs (mcMemGS := mG) .@ a) (∃ w, mapsto (hG := mc_ghG (mcMemGS := mG)) a (DfracOwn 1) w ∗ fixpoint (MinCaps_safe1 (mG := mG)) w))%I -∗
-                               ([∗ list] a ∈ (region_addrs b' e'), inv (mc_invNs (mcMemGS := mG) .@ a) (∃ w, mapsto (hG := mc_ghG (mcMemGS := mG)) a (DfracOwn 1) w ∗ fixpoint (MinCaps_safe1 (mG := mG)) w))%I.
+                                          ([∗ list] a ∈ (region_addrs b e), inv (mc_invNs (mcMemGS := mG) .@ a) (∃ w, mapsto (hG := mc_ghG (mcMemGS := mG)) a (DfracOwn 1) w ∗ fixpoint interp1 w))%I -∗
+                                                                                                                                                                                                         ([∗ list] a ∈ (region_addrs b' e'), inv (mc_invNs (mcMemGS := mG) .@ a) (∃ w, mapsto (hG := mc_ghG (mcMemGS := mG)) a (DfracOwn 1) w ∗ fixpoint interp1 w))%I.
     Proof.
       iIntros "[% %] Hregion".
       iApply (big_sepL_submseteq _ (region_addrs b' e') (region_addrs b e)).
@@ -317,29 +385,29 @@ Module MinCapsModel.
         + apply submseteq_cons; trivial.
     Qed.
 
-    Lemma safe_sub_range `{sailRegGS Σ} `{invGS Σ} {mG : memGS Σ} (b' e' b e : Addr) :
+    Lemma safe_sub_range (b' e' b e : Addr) :
       forall p a,
-      ⊢ ⌜ (b <= b')%Z /\ (e' <= e)%Z ⌝ -∗
-                               MinCaps_safe (mG := mG)
-                               (inr {| cap_permission := p; cap_begin := b; cap_end := e; cap_cursor := a |}) -∗
-                               MinCaps_safe (mG := mG)
-                               (inr {| cap_permission := p; cap_begin := b'; cap_end := e'; cap_cursor := a |}).
+        ⊢ ⌜ (b <= b')%Z /\ (e' <= e)%Z ⌝ -∗
+                                            interp
+                                            (inr {| cap_permission := p; cap_begin := b; cap_end := e; cap_cursor := a |}) -∗
+                                                                                                                              interp
+                                                                                                                              (inr {| cap_permission := p; cap_begin := b'; cap_end := e'; cap_cursor := a |}).
     Proof.
       iIntros (p a) "/= [% %] Hsafe".
-      do 2 rewrite fixpoint_MinCaps_safe1_eq.
-      destruct p; try (by iFrame); simpl; iDestruct "Hsafe" as "/= [Hsafe | %]";
+      do 2 rewrite fixpoint_interp1_eq.
+      destruct p; try (by iFrame); simpl; try iDestruct "Hsafe" as "/= [Hsafe | %]";
         try (iRight; iPureIntro; lia).
       - iLeft.
         iIntros "%".
         iAssert (⌜ (b <= e)%Z ⌝)%I as "-# Htmp".
         { iPureIntro; lia. }
         iAssert (
-          ⌜b ∈ liveAddrs ∧ e ∈ liveAddrs⌝
-                             ∗ ([∗ list] a0 ∈ region_addrs b e, inv (mc_invNs.@a0)
-                                                                    (∃ w,
-                                                                        mapsto a0 (DfracOwn 1) w
-                                                                               ∗ fixpoint MinCaps_safe1 w))
-        )%I with "[Htmp Hsafe]" as "Hsafe".
+            ⌜b ∈ liveAddrs ∧ e ∈ liveAddrs⌝
+                               ∗ ([∗ list] a0 ∈ region_addrs b e, inv (mc_invNs.@a0)
+                                                                      (∃ w,
+                                                                          mapsto a0 (DfracOwn 1) w
+                                                                                 ∗ fixpoint interp1 w))
+          )%I with "[Htmp Hsafe]" as "Hsafe".
         { iApply ("Hsafe" with "Htmp"). }
         iDestruct "Hsafe" as "[% H]".
         iSplitR.
@@ -352,12 +420,12 @@ Module MinCapsModel.
         iAssert (⌜ (b <= e)%Z ⌝)%I as "-# Htmp".
         { iPureIntro; lia. }
         iAssert (
-          ⌜b ∈ liveAddrs ∧ e ∈ liveAddrs⌝
-                             ∗ ([∗ list] a0 ∈ region_addrs b e, inv (mc_invNs.@a0)
-                                                                    (∃ w,
-                                                                        mapsto a0 (DfracOwn 1) w
-                                                                               ∗ fixpoint MinCaps_safe1 w))
-        )%I with "[Htmp Hsafe]" as "Hsafe".
+            ⌜b ∈ liveAddrs ∧ e ∈ liveAddrs⌝
+                               ∗ ([∗ list] a0 ∈ region_addrs b e, inv (mc_invNs.@a0)
+                                                                      (∃ w,
+                                                                          mapsto a0 (DfracOwn 1) w
+                                                                                 ∗ fixpoint interp1 w))
+          )%I with "[Htmp Hsafe]" as "Hsafe".
         { iApply ("Hsafe" with "Htmp"). }
         iDestruct "Hsafe" as "[% H]".
         iSplitR.
@@ -365,13 +433,17 @@ Module MinCapsModel.
           apply (le_liveAddrs H4 (conj H1 (Z.le_trans b' e' e H3 H2))).
           apply (le_liveAddrs H4 (conj (Z.le_trans b b' e' H1 H3) H2)).
         + iApply (region_addrs_submseteq $! (conj H1 H2) with "H").
-    Qed.
+      - iModIntro.
+        iDestruct "Hsafe" as "# Hsafe".
+        iModIntro.
+        admit.
+    Admitted.
 
-    Lemma specialize_range `{sailRegGS Σ} `{invGS Σ} {mG : memGS Σ} (b e addr : Addr) :
+    Lemma specialize_range (b e addr : Addr) :
       ⊢ ⌜ (b <= addr)%Z /\ (addr <= e)%Z ⌝ -∗
-        (⌜ b ∈ liveAddrs /\ e ∈ liveAddrs ⌝ ∗
-          [∗ list] a ∈ (region_addrs b e), inv (mc_invNs (mcMemGS := mG) .@ a) (∃ w, mapsto (hG := mc_ghG (mcMemGS := mG)) a (DfracOwn 1) w ∗ fixpoint (MinCaps_safe1 (mG := mG)) w))%I -∗
-        (inv (mc_invNs (mcMemGS := mG) .@ addr) (∃ w, mapsto (hG := mc_ghG (mcMemGS := mG)) addr (DfracOwn 1) w ∗ fixpoint (MinCaps_safe1 (mG := mG)) w))%I.
+                                              (⌜ b ∈ liveAddrs /\ e ∈ liveAddrs ⌝ ∗
+                                                                    [∗ list] a ∈ (region_addrs b e), inv (mc_invNs (mcMemGS := mG) .@ a) (∃ w, mapsto (hG := mc_ghG (mcMemGS := mG)) a (DfracOwn 1) w ∗ fixpoint interp1 w))%I -∗
+                                                                                                                                                                                                                                  (inv (mc_invNs (mcMemGS := mG) .@ addr) (∃ w, mapsto (hG := mc_ghG (mcMemGS := mG)) addr (DfracOwn 1) w ∗ fixpoint interp1 w))%I.
     Proof.
       iIntros "[% %] [[% %] Hrange]".
       iApply (big_sepL_elem_of with "Hrange").
@@ -379,20 +451,30 @@ Module MinCapsModel.
       split; assumption.
     Qed.
 
-    Import env.notations.
-
-    Definition luser_inst `{sailRegGS Σ} `{invGS Σ} (mG : memGS Σ) (p : Predicate) (ts : Env Val (𝑯_Ty p)) : iProp Σ :=
-      (match p return Env Val (𝑯_Ty p) -> iProp Σ with
-      | ptsreg => fun ts => MinCaps_ptsreg (env.head (env.tail ts)) (env.head ts)
-      | ptsto => fun ts => mapsto (hG := mc_ghG (mcMemGS := mG)) (env.head (env.tail ts)) (DfracOwn 1) (env.head ts)
-      | safe => fun ts => MinCaps_safe (mG := mG) (env.head ts)
-      | dummy => fun ts => True%I
-      | gprs => fun ts => interp_gprs (mG := mG)
-      end) ts.
-
-    Global Instance MinCaps_safe_Persistent `{sailRegGS Σ} `{invGS Σ} {mG : memGS Σ} (w : leibnizO MemVal) : Persistent (MinCaps_safe (mG := mG) w).
-    Proof. destruct w; simpl; rewrite fixpoint_MinCaps_safe1_eq; simpl; first apply _.
+    Global Instance interp_Persistent (w : leibnizO MemVal) : Persistent (interp w).
+    Proof. destruct w; simpl; rewrite fixpoint_interp1_eq; simpl; first apply _.
            destruct c; destruct cap_permission; apply _. Qed.
+  End Predicates.
+
+  Module MinCapsIrisPredicates <: IrisPredicates MinCapsBase MinCapsSignature MinCapsSemantics MinCapsIrisPrelims MinCapsIrisParams MinCapsIrisResources.
+    Import env.notations.
+    Import MinCapsIrisPrelims.
+    Import MinCapsIrisParams.
+    Import MinCapsIrisResources.
+    Import iris.bi.interface.
+    Import iris.bi.big_op.
+    Import iris.base_logic.lib.iprop.
+    Import iris.base_logic.lib.gen_heap.
+
+    Definition luser_inst {Σ} `{sailRegGS Σ} `{invGS Σ} (mG : memGS Σ) (p : Predicate) (ts : Env Val (𝑯_Ty p)) : iProp Σ :=
+      (match p return Env Val (𝑯_Ty p) -> iProp Σ with
+       | ptsreg     => fun ts => MinCaps_ptsreg (env.head (env.tail ts)) (env.head ts)
+       | ptsto      => fun ts => mapsto (hG := mc_ghG (mcMemGS := mG)) (env.head (env.tail ts)) (DfracOwn 1) (env.head ts)
+       | safe       => fun ts => interp (mG := mG) (env.head ts)
+       | expression => fun ts => interp_expr (mG := mG) (interp (mG := mG)) (env.head ts)
+       | dummy      => fun ts => True%I
+       | gprs       => fun ts => interp_gprs (interp (mG := mG))
+       end) ts.
 
     Definition lduplicate_inst `{sailRegGS Σ} `{invGS Σ} (mG : memGS Σ) :
       forall (p : Predicate) (ts : Env Val (𝑯_Ty p)),
@@ -401,14 +483,12 @@ Module MinCapsModel.
     Proof.
       iIntros (p ts hdup) "H".
       destruct p; inversion hdup;
-      iDestruct "H" as "#H";
-      auto.
+        iDestruct "H" as "#H";
+        auto.
     Qed.
+  End MinCapsIrisPredicates.
 
-    End WithIrisNotations.
-  End MinCapsIrisParams.
-
-  Include IrisInstance MinCapsBase MinCapsSignature MinCapsSemantics MinCapsIrisParams.
+  Include IrisInstance MinCapsBase MinCapsSignature MinCapsSemantics MinCapsIrisPrelims MinCapsIrisParams MinCapsIrisResources MinCapsIrisPredicates.
   Include ProgramLogicOn MinCapsBase MinCapsSignature MinCapsSpecification.
 
 End MinCapsModel.
@@ -419,10 +499,11 @@ Module MinCapsModel2.
   Import MinCapsSpecification.
   Import MinCapsProgram.
   Import MinCapsIrisParams.
-  Module Import MinCapsIrisModel := IrisInstanceWithContracts MinCapsBase MinCapsSignature MinCapsSpecification MinCapsSemantics MinCapsIrisParams MinCapsModel MinCapsModel.
+  Import MinCapsIrisResources.
+  Module Import MinCapsIrisModel := IrisInstanceWithContracts MinCapsBase MinCapsSignature MinCapsSpecification MinCapsSemantics MinCapsIrisPrelims MinCapsIrisParams MinCapsIrisResources MinCapsIrisPredicates MinCapsModel MinCapsModel.
 
   Section Lemmas.
-    Context `{sg : sailGS Σ}.
+    Context {Σ} `{sg : sailGS Σ}.
 
     Lemma gen_dummy_sound :
       ValidLemma lemma_gen_dummy.
@@ -470,15 +551,8 @@ Module MinCapsModel2.
       ValidLemma lemma_int_safe.
     Proof.
       intros ι. destruct_syminstance ι. cbn.
-      rewrite fixpoint_MinCaps_safe1_eq; auto.
+      rewrite fixpoint_interp1_eq; auto.
     Qed.
-
-    (* Lemma duplicate_safe_sound : *)
-    (*   ValidLemma lemma_duplicate_safe. *)
-    (* Proof. *)
-    (*   intros ι. destruct_syminstance ι. cbn. *)
-    (*   iIntros "#Hsafe". now iSplit. *)
-    (* Qed. *)
 
     Lemma safe_move_cursor_sound :
       ValidLemma lemma_safe_move_cursor.
@@ -486,10 +560,13 @@ Module MinCapsModel2.
       intros ι. destruct_syminstance ι. cbn.
       iIntros "#Hsafe".
       iSplit; [done|].
-      do 2 rewrite fixpoint_MinCaps_safe1_eq.
-      unfold MinCaps_safe1.
+      do 2 rewrite fixpoint_interp1_eq.
       destruct p; auto.
-    Qed.
+      simpl.
+      iModIntro.
+      iModIntro.
+      (* by iIntros. *)
+    Admitted.
 
     Lemma safe_sub_perm_sound :
       ValidLemma lemma_safe_sub_perm.
@@ -497,10 +574,10 @@ Module MinCapsModel2.
       intros ι. destruct_syminstance ι. cbn.
       iIntros "[#Hsafe %Hp]".
       iSplit; [done|].
-      do 2 rewrite fixpoint_MinCaps_safe1_eq.
+      do 2 rewrite fixpoint_interp1_eq.
       destruct p; destruct p'; trivial;
-        destruct Hp; discriminate.
-    Qed.
+        destruct Hp; try discriminate.
+    Admitted.
 
     Lemma safe_within_range_sound :
       ValidLemma lemma_safe_within_range.
@@ -541,13 +618,13 @@ Module MinCapsModel2.
   Lemma rM_sound `{sg : sailGS Σ} `{invGS} {Γ es δ} :
     forall a (p : Val ty.perm) (b e : Val ty.addr),
       evals es δ = env.snoc env.nil (MkB _ ty.addr) a ->
-    ⊢ semTriple δ
-        (MinCaps_safe (mG := sailGS_memGS)
-           (inr {| cap_permission := p; cap_begin := b; cap_end := e; cap_cursor := a |})
-         ∗ (⌜Subperm R p⌝ ∧ emp) ∗ ⌜(b <=? a)%Z && (a <=? e)%Z = true⌝ ∧ emp)
+      ⊢ semTriple δ
+        (interp (mG := sailGS_memGS)
+                (inr {| cap_permission := p; cap_begin := b; cap_end := e; cap_cursor := a |})
+                ∗ (⌜Subperm R p⌝ ∧ emp) ∗ ⌜(b <=? a)%Z && (a <=? e)%Z = true⌝ ∧ emp)
         (stm_foreign rM es)%env
         (λ (v : Z + Capability) (δ' : CStore Γ),
-           (MinCaps_safe (mG := sailGS_memGS) v) ∗ ⌜δ' = δ⌝).
+          (interp (mG := sailGS_memGS) v) ∗ ⌜δ' = δ⌝).
   Proof.
     intros a p b e Heq.
     iIntros "[#Hsafe [[%Hsubp _] [%Hbounds _]]]".
@@ -555,17 +632,17 @@ Module MinCapsModel2.
     rewrite wp_unfold. cbn.
     destruct p; try discriminate.
     (* TODO: clean this up! *)
-    - iAssert (inv (mc_invNs.@a) (∃ w, gen_heap.mapsto a (dfrac.DfracOwn 1) w ∗ MinCaps_safe w))%I as "Hown".
-      { rewrite fixpoint_MinCaps_safe1_eq; simpl.
+    - iAssert (inv (mc_invNs.@a) (∃ w, gen_heap.mapsto a (dfrac.DfracOwn 1) w ∗ interp w))%I as "Hown".
+      { rewrite fixpoint_interp1_eq; simpl.
         iDestruct "Hsafe" as "[Hsafe | %]"; try lia.
         iAssert (⌜ (b <= e)%Z ⌝)%I as "-# Htmp".
         { iPureIntro; lia. }
         iAssert (
-          ⌜b ∈ liveAddrs ∧ e ∈ liveAddrs⌝
-                             ∗ ([∗ list] a0 ∈ region_addrs b e,
-                                inv (mc_invNs.@a0) (∃ w, mapsto a0 (DfracOwn 1) w
-                                                        ∗ fixpoint MinCaps_safe1 w))
-        )%I with "[Htmp Hsafe]" as "Hsafe'".
+            ⌜b ∈ liveAddrs ∧ e ∈ liveAddrs⌝
+                               ∗ ([∗ list] a0 ∈ region_addrs b e,
+                                   inv (mc_invNs.@a0) (∃ w, mapsto a0 (DfracOwn 1) w
+                                                                   ∗ fixpoint interp1 w))
+          )%I with "[Htmp Hsafe]" as "Hsafe'".
         { iApply ("Hsafe" with "Htmp"). }
         iApply (specialize_range $! (conj Hb He) with "Hsafe'"). }
       iIntros (σ' ns ks1 ks nt) "[Hregs Hmem]".
@@ -586,7 +663,7 @@ Module MinCapsModel2.
       iAssert (⌜ memmap !! a = Some v ⌝)%I with "[Hav Hmem']" as "%".
       { iApply (gen_heap.gen_heap_valid with "Hmem' Hav"). }
       iMod "Hclose2" as "_".
-      iAssert (▷ (∃ v0 : Z + Capability, gen_heap.mapsto a (dfrac.DfracOwn 1) v0 ∗ fixpoint MinCaps_safe1 v0))%I with "[Hav Hrec]" as "Hinv".
+      iAssert (▷ (∃ v0 : Z + Capability, gen_heap.mapsto a (dfrac.DfracOwn 1) v0 ∗ fixpoint interp1 v0))%I with "[Hav Hrec]" as "Hinv".
       { iModIntro. iExists v. iSplitL "Hav"; iAssumption. }
       iMod ("Hclose" with "Hinv") as "_".
       iModIntro.
@@ -603,17 +680,17 @@ Module MinCapsModel2.
       apply map_Forall_lookup_1 with (i := a) (x := v) in H0; auto.
       simpl in H0. subst.
       iAssumption.
-    - iAssert (inv (mc_invNs.@a) (∃ w, gen_heap.mapsto a (dfrac.DfracOwn 1) w ∗ fixpoint (MinCaps_safe1) w))%I as "Hown".
-      { rewrite fixpoint_MinCaps_safe1_eq; simpl.
+    - iAssert (inv (mc_invNs.@a) (∃ w, gen_heap.mapsto a (dfrac.DfracOwn 1) w ∗ fixpoint (interp1) w))%I as "Hown".
+      { rewrite fixpoint_interp1_eq; simpl.
         iDestruct "Hsafe" as "[Hsafe | %]"; try lia.
         iAssert (⌜ (b <= e)%Z ⌝)%I as "-# Htmp".
         { iPureIntro; lia. }
         iAssert (
-          ⌜b ∈ liveAddrs ∧ e ∈ liveAddrs⌝
-                             ∗ ([∗ list] a0 ∈ region_addrs b e,
-                                inv (mc_invNs.@a0) (∃ w, mapsto a0 (DfracOwn 1) w
-                                                        ∗ fixpoint MinCaps_safe1 w))
-        )%I with "[Htmp Hsafe]" as "Hsafe'".
+            ⌜b ∈ liveAddrs ∧ e ∈ liveAddrs⌝
+                               ∗ ([∗ list] a0 ∈ region_addrs b e,
+                                   inv (mc_invNs.@a0) (∃ w, mapsto a0 (DfracOwn 1) w
+                                                                   ∗ fixpoint interp1 w))
+          )%I with "[Htmp Hsafe]" as "Hsafe'".
         { iApply ("Hsafe" with "Htmp"). }
         iApply (specialize_range $! (conj Hb He) with "Hsafe'"). }
       iIntros (σ' ns ks1 ks nt) "[Hregs Hmem]".
@@ -634,7 +711,7 @@ Module MinCapsModel2.
       iAssert (⌜ memmap !! a = Some v ⌝)%I with "[Hav Hmem']" as "%".
       { iApply (gen_heap.gen_heap_valid with "Hmem' Hav"). }
       iMod "Hclose2" as "_".
-      iAssert (▷ (∃ v0 : Z + Capability, gen_heap.mapsto a (dfrac.DfracOwn 1) v0 ∗ fixpoint MinCaps_safe1 v0))%I with "[Hav Hrec]" as "Hinv".
+      iAssert (▷ (∃ v0 : Z + Capability, gen_heap.mapsto a (dfrac.DfracOwn 1) v0 ∗ fixpoint interp1 v0))%I with "[Hav Hrec]" as "Hinv".
       { iModIntro. iExists v. iSplitL "Hav"; iAssumption. }
       iMod ("Hclose" with "Hinv") as "_".
       iModIntro.
@@ -651,100 +728,100 @@ Module MinCapsModel2.
       apply map_Forall_lookup_1 with (i := a) (x := v) in H0; auto.
       simpl in H0. subst.
       iAssumption.
-  Qed.
+  Admitted.
 
   Lemma wM_sound `{sg : sailGS Σ} `{invGS} {Γ es δ} :
     forall a w (p : Val ty.perm) (b e : Val ty.addr),
       evals es δ = env.snoc (env.snoc env.nil (MkB _ ty.addr) a)
                             (MkB _ ty.memval) w
-    → ⊢ semTriple δ
-        (MinCaps_safe (mG := sailGS_memGS) w
-         ∗ MinCaps_safe (mG := sailGS_memGS)
-                                          (inr {|
-                                               cap_permission := p;
-                                               cap_begin := b;
-                                               cap_end := e;
-                                               cap_cursor := a |})
-         ∗ (⌜ Subperm RW p ⌝ ∧ emp)
-         ∗ ⌜is_true ((b <=? a)%Z && (a <=? e)%Z)⌝ ∧ emp)
-        (stm_foreign wM es)
-        (λ (v3 : ()) (δ' : CStore Γ),
-         (⌜v3 = tt⌝ ∧ emp) ∗ ⌜δ' = δ⌝).
-    Proof.
-      intros a w p b e Heq.
-      iIntros "[#Hwsafe [#Hsafe [[%Hsubp _] [%Hbounds _]]]]".
-      apply andb_prop in Hbounds as [Hb%Zle_is_le_bool He%Zle_is_le_bool].
-      rewrite wp_unfold. cbn.
-      destruct p; try discriminate. clear Hsubp.
-      iIntros (σ' ns ks1 ks nt) "[Hregs Hmem]".
-      iDestruct "Hmem" as (memmap) "[Hmem' %]".
-      iAssert (inv (mc_invNs.@a) (∃ w, gen_heap.mapsto a (dfrac.DfracOwn 1) w ∗ fixpoint (MinCaps_safe1) w))%I as "Hown".
-      { do 2 rewrite fixpoint_MinCaps_safe1_eq; simpl.
-        iDestruct "Hsafe" as "[Hsafe | %]"; try lia.
-        iAssert (⌜ (b <= e)%Z ⌝)%I as "-# Htmp".
-        { iPureIntro; lia. }
-        iAssert (
+      → ⊢ semTriple δ
+          (interp (mG := sailGS_memGS) w
+                  ∗ interp (mG := sailGS_memGS)
+                  (inr {|
+                       cap_permission := p;
+                       cap_begin := b;
+                       cap_end := e;
+                       cap_cursor := a |})
+                  ∗ (⌜ Subperm RW p ⌝ ∧ emp)
+                  ∗ ⌜is_true ((b <=? a)%Z && (a <=? e)%Z)⌝ ∧ emp)
+          (stm_foreign wM es)
+          (λ (v3 : ()) (δ' : CStore Γ),
+            (⌜v3 = tt⌝ ∧ emp) ∗ ⌜δ' = δ⌝).
+  Proof.
+    intros a w p b e Heq.
+    iIntros "[#Hwsafe [#Hsafe [[%Hsubp _] [%Hbounds _]]]]".
+    apply andb_prop in Hbounds as [Hb%Zle_is_le_bool He%Zle_is_le_bool].
+    rewrite wp_unfold. cbn.
+    destruct p; try discriminate. clear Hsubp.
+    iIntros (σ' ns ks1 ks nt) "[Hregs Hmem]".
+    iDestruct "Hmem" as (memmap) "[Hmem' %]".
+    iAssert (inv (mc_invNs.@a) (∃ w, gen_heap.mapsto a (dfrac.DfracOwn 1) w ∗ fixpoint (interp1) w))%I as "Hown".
+    { do 2 rewrite fixpoint_interp1_eq; simpl.
+      iDestruct "Hsafe" as "[Hsafe | %]"; try lia.
+      iAssert (⌜ (b <= e)%Z ⌝)%I as "-# Htmp".
+      { iPureIntro; lia. }
+      iAssert (
           ⌜b ∈ liveAddrs ∧ e ∈ liveAddrs⌝
                              ∗ ([∗ list] a0 ∈ region_addrs b e,
-                                inv (mc_invNs.@a0) (∃ w, mapsto a0 (DfracOwn 1) w
-                                                        ∗ fixpoint MinCaps_safe1 w))
+                                 inv (mc_invNs.@a0) (∃ w, mapsto a0 (DfracOwn 1) w
+                                                                 ∗ fixpoint interp1 w))
         )%I with "[Htmp Hsafe]" as "Hsafe'".
-        { iApply ("Hsafe" with "Htmp"). }
-        iApply (specialize_range $! (conj Hb He) with "Hsafe'"). }
-      iInv "Hown" as "Hinv" "Hclose".
-      iMod (fupd_mask_subseteq empty) as "Hclose2"; first set_solver.
-      iModIntro.
-      iSplitR; first by intuition.
-      iIntros (e2 σ'' efs) "%".
-      dependent elimination H1.
-      dependent elimination s.
-      rewrite Heq in f1.
-      cbn in f1.
-      dependent elimination f1.
-      do 3 iModIntro.
-      iDestruct "Hinv" as (v) "Hav".
-      iDestruct "Hav" as "[Hav Hrec]".
-      iMod (gen_heap.gen_heap_update _ _ _ w with "Hmem' Hav") as "[Hmem' Hav]".
-      iMod "Hclose2" as "_".
-      iAssert (▷ (∃ v0 : Z + Capability, gen_heap.mapsto a (dfrac.DfracOwn 1) v0 ∗ fixpoint MinCaps_safe1 v0))%I with "[Hav Hrec]" as "Hinv".
-      { iModIntro. iExists w. iSplitL "Hav"; iAssumption. }
-      iMod ("Hclose" with "Hinv") as "_".
-      iModIntro.
-      iSplitL; trivial.
-      cbn.
-      iSplitL "Hregs"; first by iFrame.
-      - iExists (<[a:=w]> memmap).
-        iSplitL; first by iFrame.
-        iPureIntro.
-          apply map_Forall_lookup.
-          intros i x Hl.
-          unfold fun_wM.
-          cbn in *.
-          destruct (Z.eqb a i) eqn:Heqb.
-          + rewrite -> Z.eqb_eq in Heqb.
-            subst.
-            apply (lookup_insert_rev memmap i); assumption.
-          + rewrite -> map_Forall_lookup in H0.
-            rewrite -> Z.eqb_neq in Heqb.
-            rewrite -> (lookup_insert_ne _ _ _ _ Heqb) in Hl.
-            apply H0; assumption.
-      - iSplitL; trivial.
-        iApply wp_value; cbn; trivial;
-          repeat (iSplitL; trivial).
-    Qed.
-
-  Lemma foreignSem : ForeignSem.
-  Proof.
-    intros Γ τ Δ f es δ.
-    destruct f; cbn - [MinCaps_safe MinCaps_csafe];
-      intros ι; destruct_syminstance ι;
-        eauto using dI_sound, rM_sound, wM_sound.
+      { iApply ("Hsafe" with "Htmp"). }
+      iApply (specialize_range $! (conj Hb He) with "Hsafe'"). }
+    iInv "Hown" as "Hinv" "Hclose".
+    iMod (fupd_mask_subseteq empty) as "Hclose2"; first set_solver.
+    iModIntro.
+    iSplitR; first by intuition.
+    iIntros (e2 σ'' efs) "%".
+    dependent elimination H1.
+    dependent elimination s.
+    rewrite Heq in f1.
+    cbn in f1.
+    dependent elimination f1.
+    do 3 iModIntro.
+    iDestruct "Hinv" as (v) "Hav".
+    iDestruct "Hav" as "[Hav Hrec]".
+    iMod (gen_heap.gen_heap_update _ _ _ w with "Hmem' Hav") as "[Hmem' Hav]".
+    iMod "Hclose2" as "_".
+    iAssert (▷ (∃ v0 : Z + Capability, gen_heap.mapsto a (dfrac.DfracOwn 1) v0 ∗ fixpoint interp1 v0))%I with "[Hav Hrec]" as "Hinv".
+    { iModIntro. iExists w. iSplitL "Hav"; iAssumption. }
+    iMod ("Hclose" with "Hinv") as "_".
+    iModIntro.
+    iSplitL; trivial.
+    cbn.
+    iSplitL "Hregs"; first by iFrame.
+    - iExists (<[a:=w]> memmap).
+      iSplitL; first by iFrame.
+      iPureIntro.
+      apply map_Forall_lookup.
+      intros i x Hl.
+      unfold fun_wM.
+      cbn in *.
+      destruct (Z.eqb a i) eqn:Heqb.
+      + rewrite -> Z.eqb_eq in Heqb.
+        subst.
+        apply (lookup_insert_rev memmap i); assumption.
+      + rewrite -> map_Forall_lookup in H0.
+        rewrite -> Z.eqb_neq in Heqb.
+        rewrite -> (lookup_insert_ne _ _ _ _ Heqb) in Hl.
+        apply H0; assumption.
+    - iSplitL; trivial.
+      iApply wp_value; cbn; trivial;
+        repeat (iSplitL; trivial).
   Qed.
 
-  Lemma lemSem : LemmaSem.
+  Lemma foreignSem `{sg : sailGS Σ} : ForeignSem.
+  Proof.
+    intros Γ τ Δ f es δ.
+    destruct f; cbn - [interp];
+      intros ι; destruct_syminstance ι;
+      eauto using dI_sound, rM_sound, wM_sound.
+  Qed.
+
+  Lemma lemSem `{sg : sailGS Σ} : LemmaSem.
   Proof.
     intros Δ []; eauto using
-      open_ptsreg_sound, close_ptsreg_sound,
+                       open_ptsreg_sound, close_ptsreg_sound,
       open_gprs_sound, close_gprs_sound, int_safe_sound,
       safe_move_cursor_sound, safe_sub_perm_sound,
       safe_within_range_sound, gen_dummy_sound.
